common/Smallstep.v
@@ -127,6 +127,15 @@ Proof.
   eauto.
 Qed.
 
+Lemma inv_star:
+  forall ge (P: _ -> Prop),
+    (forall s1 t s2, step ge s1 t s2 -> P s1 -> P s2) ->
+    forall s1 t s2, star ge s1 t s2 -> P s1 -> P s2.
+Proof.
+  intros ge P INV.
+  induction 1; simpl; intros; eauto.
+Qed.
+
 (** One or several transitions.  Also known as the transitive closure. *)
 
 Inductive plus (ge: genv): state -> trace -> state -> Prop :=
@@ -270,6 +279,16 @@ Lemma plus_E0_ind:
   forall s1 s2, plus ge s1 E0 s2 -> P s1 s2.
 Proof.
   intros. inv H0. exploit Eapp_E0_inv; eauto. intros [A B]; subst. eauto.
+Qed.
+
+Lemma inv_plus:
+  forall ge (P: _ -> Prop),
+    (forall s1 t s2, step ge s1 t s2 -> P s1 -> P s2) ->
+    forall s1 t s2, plus ge s1 t s2 -> P s1 -> P s2.
+Proof.
+  intros ge P INV s1 t s2 PLUS PS1.
+  inv PLUS.
+  eapply inv_star; eauto.
 Qed.
 
 (** Counted sequences of transitions *)
